rich

theories/SLFRich.v
@@ -4,81 +4,725 @@ Separation Logic Foundations
 
 Chapter: "Rich".
 
-This chapter describes extension to the Separation Logic foundations
-for dealing with richer language constructs, including records, arrays,
-loops, data constructors, pattern matching, null pointers, as well as
-terms that are not in A-normal form, and support for linear (non-affine)
-resources.
-
 Author: Arthur Charguéraud.
 License: CC-by 4.0.
 
 *)
 
+Set Implicit Arguments.
+From Sep Require Import SLFExtra TLCbuffer.
+
+Implicit Types P : Prop.
+Implicit Types H : hprop.
+Implicit Types Q : val->hprop.
+Implicit Type p q : loc.
+Implicit Type k : nat.
+Implicit Type i n : int.
+Implicit Type v : val.
+Implicit Types b : bool.
+
+
 (* ####################################################### *)
 (** * Chapter in a rush *)
 
-(* ******************************************************* *)
-(** ** Records *)
+(** This chapter introduces support for additional language constructs:
+    - while-loops and for-loops,
+    - assertions,
+    - n-ary functions.
 
-(* ******************************************************* *)
-(** ** Arrays *)
+    Regarding loops, we explain why conventional-style reasoning rules
+    based on loop invariants are limited in that they prevent useful
+    applications of the frame rule. We present alternative reasoning rules
+    compatible with the frame rule, and demonstrate their benefits on
+    practical examples.
+
+    Regarding assertions, we present a reasoning rule such that:
+    - assertions may be expressed in terms of mutable data, and possibly
+      to perform local side-effects, and
+    - the program remains correct whether assertions are executed or not.
+
+    Regarding n-ary functions, that is, functions with several arguments
+    there are essentially three possible approaches:
+
+    - native n-ary functions, e.g., [function(x, y) { t } ] in C syntax;
+    - curried functions, e.g., [fun x => fun y => t] in OCaml syntax;
+    - tupled functions, e.g., [fun (x,y) => t] in OCaml syntax.
+
+    In this chapter, we present reasoning rules for curried functions and
+    for native n-ary functions. The former requires minimal extension to the
+    syntax and semantics of our language. The latter corresponds to the most
+    practical solution from an engineering perspective.
+
+*)
+
+
+(* ####################################################### *)
+(** ** If with a term as condition *)
+
+Parameter eval_if_trm : forall s1 s2 s3 v b t0 t1 t2,
+  eval s1 t0 s2 (val_bool b) ->
+  eval s2 (if b then t1 else t2) s3 v ->
+  eval s1 (trm_if t0 t1 t2) s3 v.
 
 
 
+Lemma hoare_if_trm : forall (Q':bool->hprop) t0 t1 t2 H Q,
+  hoare t0 H (fun r => \exists b, \[r = b] \* Q' b) ->
+  (forall b, hoare (if b then t1 else t2) (Q' b) Q) ->
+  hoare (trm_if t0 t1 t2) H Q.
+Proof using.
+  introv M1 M2. intros s1 K1. lets (s2&v0&R2&K2'): M1 K1.
+  lets (b'&K2): hexists_inv K2'. rewrite hstar_hpure in K2.
+  destruct K2 as (->&K2).
+  forwards (s3&v&R&K): M2 K2. exists s3 v. splits.
+  { applys eval_if_trm R2 R. }
+  { applys K. }
+Qed.
+
+Lemma triple_if_trm : forall (Q':bool->hprop) t0 t1 t2 H Q,
+  triple t0 H (fun r => \exists b, \[r = b] \* Q' b) ->
+  (forall b, triple (if b then t1 else t2) (Q' b) Q) ->
+  triple (trm_if t0 t1 t2) H Q.
+Proof using.
+  introv M1 M2. intros HF. applys hoare_if_trm (fun b => Q' b \* HF).
+  { applys hoare_conseq. applys M1 HF. { xsimpl. } { xsimpl. auto. } }
+  { intros v. applys M2. }
+Qed.
 
 
+(* ####################################################### *)
+(** ** Limitation of loop invariants in Separation Logic *)
+
+
+(* ####################################################### *)
+(** ** Separation-Logic-friendly reasoning rule for while-loops *)
+
+Module WhileLoops.
+
+Parameter trm_while : trm -> trm -> trm.
+
+Parameter eval_while : forall s1 s2 t1 t2 v,
+  eval s1 (trm_if t1 (trm_seq t2 (trm_while t1 t2)) val_unit) s2 v ->
+  eval s1 (trm_while t1 t2) s2 v.
+
+Lemma hoare_while_raw : forall t1 t2 H Q,
+  hoare (trm_if t1 (trm_seq t2 (trm_while t1 t2)) val_unit) H Q ->
+  hoare (trm_while t1 t2) H Q.
+Proof using.
+  introv M K. forwards* (s'&v&R1&K1): M.
+  exists s' v. splits*. { applys* eval_while. }
+Qed.
+
+Lemma triple_while : forall t1 t2 H Q,
+  triple (trm_if t1 (trm_seq t2 (trm_while t1 t2)) val_unit) H Q ->
+  triple (trm_while t1 t2) H Q.
+Proof using.
+  introv M. intros H'. apply hoare_while_raw. applys* M.
+Qed.
+
+Lemma triple_while_abstract : forall t1 t2 H Q,
+  (forall t,
+     (forall H' Q', triple (trm_if t1 (trm_seq t2 t) val_unit) H' Q' ->
+                    triple t H' Q') ->
+    triple t H Q) ->
+  triple (trm_while t1 t2) H Q.
+Proof using.
+  introv M. applys M. introv K. applys triple_while. applys K.
+Qed.
+
+
+Lemma triple_while_inv_not_framable : forall (A:Type) (I:bool->A->hprop) (R:A->A->Prop) t1 t2,
+  wf R ->
+  (forall b X, triple t1 (I b X) (fun r => \exists b', \[r = b'] \* I b' X)) ->
+  (forall b X, triple t2 (I b X) (fun _ => \exists b' Y, \[R Y X] \* I b' Y)) ->
+  triple (trm_while t1 t2) (\exists b X, I b X) (fun r => \exists Y, I false Y).
+Proof using.
+  introv WR M1 M2. applys triple_hexists. intros b. applys triple_hexists. intros X.
+  gen b. induction_wf IH: WR X. intros. applys triple_while.
+  applys triple_if_trm (fun b' => I b' X).
+  { applys M1. }
+  { intros b'. case_if.
+    { applys triple_seq.
+      { applys M2. }
+      { applys triple_hexists. intros b''. applys triple_hexists. intros Y.
+        applys triple_hpure. intros HR. applys IH HR. } }
+    { applys triple_val. xsimpl. } }
+Qed.
+
+Lemma triple_while_inv : forall (A:Type) (I:bool->A->hprop) (R:A->A->Prop) t1 t2,
+  let Q := (fun r => \exists Y, I false Y) in
+  wf R ->
+  (forall t b X, 
+    (forall b' Y, R Y X -> triple t (I b' Y) Q) ->
+    triple (trm_if t1 (trm_seq t2 t) val_unit) (I b X) Q) ->
+  triple (trm_while t1 t2) (\exists b X, I b X) Q.
+Proof using.
+  introv WR M. applys triple_hexists. intros b0. applys triple_hexists. intros X0.
+  gen b0. induction_wf IH: WR X0. intros. applys triple_while.
+  applys M. intros b' Y HR'. applys IH HR'.
+Qed.
+
+Lemma triple_while_inv_conseq_frame : forall (A:Type) (I:bool->A->hprop) (R:A->A->Prop) H' t1 t2 H Q,
+  let Q' := (fun r => \exists Y, I false Y) in
+  wf R ->
+  (H ==> (\exists b X, I b X) \* H') ->
+  (forall t b X,
+      (forall b' Y, R Y X -> triple t (I b' Y) Q') ->
+      triple (trm_if t1 (trm_seq t2 t) val_unit) (I b X) Q') ->
+  Q' \*+ H' ===> Q (* add [\*+ \GC] for affine logic *) ->
+  triple (trm_while t1 t2) H Q.
+Proof using.
+  introv WR WH M WQ. applys triple_conseq_frame WH WQ.
+  applys triple_while_inv WR M.
+Qed.
+
+
+Parameter triple_conseq_frame_hgc : forall H2 H1 Q1 t H Q,
+  triple t H1 Q1 ->
+  H ==> H1 \* H2 ->
+  Q1 \*+ H2 ===> Q \*+ \GC ->
+  triple t H Q.
+
+Lemma triple_while_inv_conseq_frame_gc : forall (A:Type) (I:bool->A->hprop) (R:A->A->Prop) H' t1 t2 H Q,
+  let Q' := (fun r => \exists Y, I false Y) in
+  wf R ->
+  (H ==> (\exists b X, I b X) \* H') ->
+  (forall t b X,
+      (forall b' Y, R Y X -> triple t (I b' Y) Q') ->
+      triple (trm_if t1 (trm_seq t2 t) val_unit) (I b X) Q') ->
+  Q' \*+ H' ===> Q \*+ \GC ->
+  triple (trm_while t1 t2) H Q.
+Proof using.
+  introv WR WH M WQ. applys triple_conseq_frame_hgc WH WQ.
+  applys triple_while_inv WR M.
+Qed.
+
+
+Lemma wp_while_inv_conseq : forall (A:Type) (I:bool->A->hprop) (R:A->A->Prop) t1 t2,
+  let Q := (fun r => \exists Y, I false Y) in
+  wf R ->
+     (\exists b X, I b X)
+  \* \[forall t b X,
+      (forall b' Y, R Y X -> (I b' Y) ==> wp t Q) ->
+       (I b X) ==> wp (trm_if t1 (trm_seq t2 t) val_unit) Q]
+   ==> wp (trm_while t1 t2) Q.
+Proof using.
+  introv WR. sets H: (\exists b X, I b X). xpull. intros M.
+  rewrite wp_equiv. applys triple_while_inv WR.
+  introv N. rewrite <- wp_equiv. applys M. 
+  introv HR. rewrite wp_equiv. applys N HR.
+Qed.
+
+End WhileLoops.
 
 
 
 (* ####################################################### *)
-(** * Details *)
+(** ** Reasoning rule for for-loops *)
 
 
+(* ####################################################### *)
+(** ** Reasoning rule for assertions *)
 
-Arguments qwand_cancel [A].
+Module Assertions.
 
-(** A conditional of the form [if t0 then t1 else t2] can
-    be encoded as [let x = t0 in if x then t1 else t2].
-    Thus, assuming programs to be written in A-normal form
-    (i.e., with arguments of conditionals and applications
-    restricted to variables and values), one could live
-    without a reasoning rule for [if t0 then t1 else t2].
-    Nevertheless, to support reasoning about programs that
-    are not written in A-normal form, we present more general
-    rules further in this chapter. *)
+Parameter val_assert : prim.
 
-(** Remark: our language is set up in such a way that a non-recursive
-    function is just a special case of a (potentially-recursive) function.
-    The term [trm_fix z x t1] denotes a potentially-recursive function,
-    where [z] is a binder. This binder may be either a variable [f],
-    in the case of a recursive function, or the special anonymous binder
-    written [bind_anon] to denote a non-recursive function. *)
+Parameter eval_assert : forall s t s',
+  eval s t s' (val_bool true) ->
+  eval s (val_assert t) s' val_unit.
 
-Check trm_fix : bind -> var -> trm -> trm.
+Parameter eval_assert_ignore : forall s t,
+  eval s (val_assert t) s val_unit.
 
-Definition trm_fun' x t1 := trm_fix bind_anon x t1.
+Parameter eval_assert_both : forall s t s' v, (* too restrictive *)
+  eval s t s' v ->
+  eval s val_unit s' v ->
+  eval s (val_assert t) s' v.
 
-(* null pointers *)
+Lemma hoare_assert : forall t H,
+  hoare t H (fun r => \[r = true] \* H) ->
+  hoare (val_assert t) H (fun _ => H).
+Proof using.
+  introv M. intros s K. forwards (s'&v&R&N): M K.
+  rewrite hstar_hpure in N. destruct N as (->&K').
+  exists s' val_unit. split. 
+  { applys eval_assert R. }
+  { applys K'. }
+Qed.
 
+Lemma triple_assert : forall t H,
+  triple t H (fun r => \[r = true] \* H) ->
+  triple (val_assert t) H (fun _ => H).
+Proof using.
+  introv M. intros H'. specializes M H'. applys hoare_assert. 
+  applys hoare_conseq M. { xsimpl. } { xsimpl. auto. }
+Qed.
 
-
-
-Notation "'TRIPLE' t 'PRE' H1 'BIND' x1 x2 x3 'RET' v 'POST' H2" :=
-  (forall Q, H1 \* \[forall x1 x2 x3, H2 ==> Q v] ==> WP t Q)
-  (at level 68, t at level 0, x1 ident, x2 ident, x3 ident) : triple_scope.
-
-Notation "'TRIPLE' t 'PRE' H1 'RET' v 'POST' H2" :=
-  (forall Q, H1 \* \[(fun r => \[r = v] \* H2) ===> Q] ==> WP t Q)
-  (at level 39, t at level 0) : triple_scope.
-
-
-Notation "'\exists' x1 .. xn , H" :=
-  (hexists (fun x1 => .. (hexists (fun xn => H)) ..))
-  (at level 39, x1 binder, H at level 50, right associativity,
-   format "'[' '\exists' '/ '  x1  ..  xn , '/ '  H ']'").
+End Assertions.
 
 
+(* ####################################################### *)
+(** ** Curried functions of several arguments *)
 
+Module CurriedFun.
+Open Scope liblist_scope.
+Implicit Types f : var.
+
+(** We next give a quick presentation of the notation, lemmas and
+    tactics involved in the manipulation of curried functions of
+    several arguments.
+
+    We focus here on the particular case of recursive functions with 2
+    arguments, to illustrate the principles. Set up for non-recursive and
+    recursive functions of arity 2 and 3 can be found in the file [SLFExtra].
+    One may attempt to generalize these definitions to handle arbitrary
+    arities. Yet, to obtain an arity-generic treatment of functions, it is
+    much simpler to work with primitive n-ary functions, whose treatment is
+    presented further on.
+
+    Consider a curried recursive functions that expects two arguments.
+    [val_fix f x1 (trm_fun x2 t)] describes such a function, where [f]
+    denotes the name of the function for recursive calls, [x1] and [x2]
+    denote the arguments, and [t] denotes the body. Observe that the
+    inner function, the one that expects [x2], is not recursive, and that
+    it is not a value but a term (because it may refer to the variable [x1]
+    bound outside of it).
+
+    We introduce the notation [Fix f x1 x2 := t] to generalize the notation
+    [Fix f x := t] to the case of a recursive function of two arguments. *)
+
+Notation "'Fix' f x1 x2 ':=' t" :=
+  (val_fix f x1 (trm_fun x2 t))
+  (at level 69, f, x1, x2 at level 0,
+  format "'Fix'  f  x1  x2  ':='  t").
+
+(** An application of a function of two arguments takes the form
+    [f v1 v2], which is actually parsed as [trm_app (trm_app f v1) v2].
+
+    This expression is an application of a term to a value, and not of
+    a value to a value. Thus, this expression cannot be evaluated using
+    the rule [eval_app_fun]. We need a distinct rule for first evaluating
+    the arguments of a function application to values, before we can
+    evaluate the application of a value to a value.
+
+    The rule [eval_app_args] serves that purpose. To state it, we first
+    need to characterize whether a term is a value or not, using the
+    predicate [trm_is_val t] defined next. *)
+
+Definition trm_is_val (t:trm) : Prop :=
+  match t with trm_val v => True | _ => False end.
+
+(** The statement of [eval_app_args] then takes the following form.
+    For an expression [trm_app t1 t2] where either [t1] or [t2] is
+    not a value, it enables reducing both [t1] and [t2] to values,
+    leaving a premise of the form [trm_app v1 v2], which is subject
+    to the rule [eval_app_fun] for evaluating functions. *)
+
+Parameter eval_app_args : forall s1 s2 s3 s4 t1 t2 v1 v2 r,
+  (~ trm_is_val t1 \/ ~ trm_is_val t2) ->
+  eval s1 t1 s2 v1 ->
+  eval s2 t2 s3 v2 ->
+  eval s3 (trm_app v1 v2) s4 r ->
+  eval s1 (trm_app t1 t2) s4 r.
+
+(** Using this rule, we can establish an evaluation rule for the
+    term [v0 v1 v2]. There, [v0] is a recursive function of two
+    arguments named [x1] and [x2], the values [v1] and [v2] denote
+    the corresponding arguments, and [f] denotes the name of the
+    function available for making recursive calls from the body [t1].
+
+    The key idea is that the behavior of [v0 v1 v2] is similar to
+    that of the term [subst x2 v2 (subst x1 v1 (subst f v0 t1))].
+    We state this property using the predicate [eval_like], introduced
+    in the chapter [SLFRules]. *)
+
+Lemma eval_like_app_fix2 : forall v0 v1 v2 f x1 x2 t1,
+  v0 = val_fix f x1 (trm_fun x2 t1) ->
+  (x1 <> x2 /\ f <> x2) ->
+  eval_like (subst x2 v2 (subst x1 v1 (subst f v0 t1))) (v0 v1 v2).
+Proof using.
+  introv E (N1&N2). introv R. applys* eval_app_args.
+  { applys eval_app_fix E. simpl. do 2 (rewrite var_eq_spec; case_if).
+    applys eval_fun. }
+  { applys* eval_val. }
+  { applys* eval_app_fun. }
+Qed.
+
+(** From this result, we can easily prove the specification triple
+    for applications of the form [v0 v1 v2]. *)
+
+Lemma triple_app_fix2 : forall f x1 x2 v0 v1 v2 t1 H Q,
+  v0 = val_fix f x1 (trm_fun x2 t1) ->
+  (x1 <> x2 /\ f <> x2) ->
+  triple (subst x2 v2 (subst x1 v1 (subst f v0 t1))) H Q ->
+  triple (v0 v1 v2) H Q.
+Proof using.
+  introv E N M1. applys triple_eval_like M1. applys* eval_like_app_fix2.
+Qed.
+
+(** We can exploit the same result to esablish the corresponding
+    weakest-precondition style version of the reasoning rule. *)
+
+Lemma wp_app_fix2 : forall f x1 x2 v0 v1 v2 t1 Q,
+  v0 = val_fix f x1 (trm_fun x2 t1) ->
+  (x1 <> x2 /\ f <> x2) ->
+  wp (subst x2 v2 (subst x1 v1 (subst f v0 t1))) Q ==> wp (trm_app v0 v1 v2) Q.
+Proof using. introv EQ1 N. applys wp_eval_like. applys* eval_like_app_fix2. Qed.
+
+(** We can then reformulate this wp-style rule in a way that suits
+    the needs of the [xwp] tactic, using a conclusion expressed
+    using a [triple], and using a premise expressed using [wpgen].
+    Observe the substitution context, which is instantiated as
+    [(f,v0)::(x1,v1)::(x2,v2)::nil]. Note also how the side-conditions
+    expressing the fact that the variables are distinct are stated
+    using a comparison function for variables that computes in Coq. *)
+
+Lemma xwp_lemma_fix2 : forall f v0 v1 v2 x1 x2 t H Q,
+  v0 = val_fix f x1 (trm_fun x2 t) ->
+  (var_eq x1 x2 = false /\ var_eq f x2 = false) ->
+  H ==> wpgen ((f,v0)::(x1,v1)::(x2,v2)::nil) t Q ->
+  triple (v0 v1 v2) H Q.
+Proof using.
+  introv M1 N M2. repeat rewrite var_eq_spec in N. rew_bool_eq in *.
+  rewrite <- wp_equiv. xchange M2.
+  xchange (>> wpgen_sound (((f,v0)::nil) ++ ((x1,v1)::nil) ++ ((x2,v2)::nil)) t Q).
+  do 2 rewrite isubst_app. do 3 rewrite <- subst_eq_isubst_one.
+  applys* wp_app_fix2.
+Qed.
+
+(** Finally, we can generalize the [xwp] tactic by integrating in
+    its implementation an attempt to invoke the above lemma. *)
+
+Tactic Notation "xwp" :=
+  intros;
+  first [ applys xwp_lemma_fun; [ reflexivity | ]
+        | applys xwp_lemma_fix; [ reflexivity | ]
+        | applys xwp_lemma_fix2; [ reflexivity | splits; reflexivity | ] ];
+  xwp_simpl.
+
+(** The generalized version of [xwp] following this line is
+    formalized in the file [SLFExtra.v] and was put to practice
+    in several examples from the chapter [SLFBasic]. *)
+
+End CurriedFun.
+
+
+(* ####################################################### *)
+(** ** Primitive n-ary functions *)
+
+Module PrimitiveNaryFun.
+
+(** We next present an alternative treatment to functions of several
+    arguments. The idea is to represent arguments using lists.
+
+    On the one hand, the manipulation of lists adds a little bit of
+    boilerplate. On the other hand, when using this representation, all
+    the definitions and lemmas are inherently arity-generic, that is,
+    they work for any number of arguments.
+
+    We introduce the short names [vars], [vals] and [trms] to denote lists
+    of variables, lists of values, and lists of terms, respectively.
+    These names are not only useful to improve conciseness, they also enable
+    the set up of useful coercions, as we will detail shortly afterwards. *)
+
+Definition vars : Type := list var.
+Definition vals : Type := list val.
+Definition trms : Type := list trm.
+
+Implicit Types xs : vars.
+Implicit Types vs : vals.
+Implicit Types ts : trms.
+
+(** We assume the grammar of terms and values to include primitive n-ary
+    functions and n-ary applications, featuring list of arguments.
+    Thereafter, for conciseness, we omit non-recursive functions, and
+    focus on the treatment of the more-general recursive functions. *)
+
+Parameter val_fixs : var -> vars -> trm -> val.
+Parameter trm_fixs : var -> vars -> trm -> trm.
+Parameter trm_apps : trm -> trms -> trm.
+
+(** The substitution function is a bit tricky to update for dealing with
+    list of variables. A definition along the following lines works well.
+    On the one hand, it prevents variables capture. On the other hand,
+    it traverses recursively the list of arguments, in a way that is
+    recognized as structurally recursive.
+
+[[
+    Fixpoint subst (y:var) (w:val) (t:trm) : trm :=
+      let aux t := (subst y w t) in
+      let aux_no_captures xs t := (If List.In y xs then t else aux t) in
+      match t with
+      | trm_fixs f xs t1 => trm_fixs f xs (If f = y then t1 else
+                                            aux_no_captures xs t1)
+      | trm_apps t0 ts => trm_apps (aux t0) (List.map aux ts)
+      ...
+     end.
+]]
+
+    For additional details, we refer to the implementation of CFML.
+*)
+
+(** The evaluation rules need to be updated accordingly. A n-ary function
+    from the grammar of terms evaluates to the corresponding n-ary
+    function from the grammar of values. For technical reasons, we
+    need to ensure that the program is well-formed and that the list
+    of arguments to the function is nonempty. Indeed, a function of
+    zero arguments is not considered a function in our language.
+    (Otherwise, such a function [f] would beta-reduce to its body
+    as soon as it is defined, because it waits for no arguments.) *)
+
+Parameter eval_fixs : forall m f xs t1,
+  xs <> nil ->
+  eval m (trm_fixs f xs t1) m (val_fixs f xs t1).
+
+(** The application of a n-ary function to values takes the form
+    [trm_apps (trm_val v0) ((trm_val v1):: .. ::(trm_val vn)::nil)].
+    If the function [v0] is defined as [val_fixs f xs t1], where [xs]
+    denotes the list [x1::x2::...::xn::nil], then the beta-reduction
+    of the function application triggers the evaluation of the
+    substitution [subst xn vn (... (subst x1 v1 (subst f v0 t1)) ...)].
+
+    To describe the evaluation rule in an arity-generic way, we need to
+    introduce the list [vs] made of the values provided as arguments,
+    that is, the list [v1::v2::..::vn::nil].
+
+    With this list [vs], the n-ary application can then be written as the
+    term [trm_apps (trm_val v0) (trms_vals vs)], where the operation
+    [trms_vals] converts a list of values into a list of terms by
+    applying the constructor [trm_val] to every value from the list. *)
+
+Coercion trms_vals (vs:vals) : trms :=
+  LibList.map trm_val vs.
+
+(** Note that we declare the operation [trms_vals] as a coercion, just
+    like [trm_val] is a coercion. Doing so enables us to write a n-ary
+    application in the form [v0 vs]. *)
+
+(** To describe the iterated substitution
+    [subst xn vn (... (subst x1 v1 (subst f v0 t1)) ...)], we introduce
+    the operation [substn xs vs t], which substitutes the variables [xs]
+    with the values [vs] inside the [t]. It is defined recursively,
+    by iterating calls to the function [subst] for substituting the
+    variables one by one. *)
+
+Fixpoint substn (xs:list var) (vs:list val) (t:trm) : trm :=
+  match xs,vs with
+  | x::xs', v::vs' => substn xs' vs' (subst x v t)
+  | _,_ => t
+  end.
+
+(** This substitution operation is well-behaved only if the list [xs]
+    and the list [vs] have the same lengths. It is also desirable for
+    reasoning about the evaluation rule to guarantee that the list of
+    variables [xs] contains variables that are distinct from each others
+    and distinct from [f], and to guarantee that the list [xs] is not empty.
+
+    To formally capture all these invariants, we introduce the predicate
+    [var_fixs f xs n], where [n] denotes the number of arguments the
+    function is being applied to. Typically, [n] is equal to the length
+    of the list of arguments [vs]). *)
+
+Definition var_fixs (f:var) (xs:vars) (n:nat) : Prop :=
+     LibList.noduplicates (f::xs)
+  /\ length xs = n
+  /\ xs <> nil.
+
+(** The evaluation of a recursive function [v0] defined as [val_fixs f xs t1]
+    on a list of arguments [vs] triggers the evaluation of the term
+    [substn xs vs (subst f v0 t1)], same as [substn (f::xs) (v0::vs) t1].
+    The evaluation rule is stated as follows, using the predicate [var_fixs]
+    to enforce the appropriate invariants on the variable names. *)
+
+Parameter eval_apps_fixs : forall v0 vs f xs t1 s1 s2 r,
+  v0 = val_fixs f xs t1 ->
+  var_fixs f xs (LibList.length vs) ->
+  eval s1 (substn (f::xs) (v0::vs) t1) s2 r ->
+  eval s1 (trm_apps v0 (trms_vals vs)) s2 r.
+
+(** The corresponding reasoning rule has a somewhat similar statement. *)
+
+Lemma triple_apps_fixs : forall v0 vs f xs t1 H Q,
+  v0 = val_fixs f xs t1 ->
+  var_fixs f xs (LibList.length vs)->
+  triple (substn (f::xs) (v0::vs) t1) H Q ->
+  triple (trm_apps v0 vs) H Q.
+Proof using.
+  introv E N M. applys triple_eval_like M.
+  introv R. applys* eval_apps_fixs.
+Qed.
+
+(** The statement of the above lemma applies only to terms that are
+    of the form [trm_apps (trm_val v0) (trms_vals vs)]. Yet, in practice,
+    goals are generally of the form
+    [trm_apps (trm_val v0) ((trm_val v1):: .. :: (trm_val vn)::nil)].
+    The two forms are convertible, yet in general Coq is not able to
+    synthetize the list [vs] during the unification process.
+
+    Fortunately, it is possible to reformulate the lemma using an auxiliary
+    conversion function named [trms_to_vals], whose evaluation by Coq's
+    unification process is able to synthetize the list [vs].
+
+    The operation [trms_to_vals ts], if all the terms in [ts] are of the
+    form [trm_val vi], returns a list of values [vs] such that [ts] is
+    equal to [trms_vals vs]. Otherwise, the operation returns [None].
+    The definition and specification of the operation [trms_to_vals]
+    are as follows. *)
+
+Fixpoint trms_to_vals (ts:trms) : option vals :=
+  match ts with
+  | nil => Some nil
+  | (trm_val v)::ts' =>
+      match trms_to_vals ts' with
+      | None => None
+      | Some vs' => Some (v::vs')
+      end
+  | _ => None
+  end.
+
+Lemma trms_to_vals_spec : forall ts vs,
+  trms_to_vals ts = Some vs ->
+  ts = trms_vals vs.
+Proof using.
+  intros ts. induction ts as [|t ts']; simpl; introv E.
+  { inverts E. auto. }
+  { destruct t; inverts E as E. cases (trms_to_vals ts') as C; inverts E.
+    rename v0 into vs'. rewrite* (IHts' vs'). }
+Qed.
+
+Lemma demo_trms_to_vals : forall v1 v2 v3,
+  exists vs,
+     trms_to_vals ((trm_val v1)::(trm_val v2)::(trm_val v3)::nil) = Some vs
+  /\ vs = vs.
+Proof using.
+  (* activate the display of coercions to play this demo *)
+  intros. esplit. split. simpl. eauto. (* [vs] was inferred. *)
+Abort.
+
+(** Using [trms_to_vals], we can reformulate [triple_apps_fixs'] in such
+    a way that the rule can be smoothly applied on practical goals. *)
+
+Lemma triple_apps_fixs' : forall v0 ts vs f xs t1 H Q,
+  v0 = val_fixs f xs t1 ->
+  trms_to_vals ts = Some vs ->
+  var_fixs f xs (LibList.length vs)->
+  triple (substn (f::xs) (v0::vs) t1) H Q ->
+  triple (trm_apps v0 ts) H Q.
+Proof using.
+  introv E T N M. rewrites (@trms_to_vals_spec _ _ T).
+  applys* triple_apps_fixs.
+Qed.
+
+(** To set up the tactic [xwp] to handle n-ary applications, we reformulate
+    the lemma above by making two changes.
+
+    The first change is to replace the predicate [var_fixs] which checks
+    the well-formedness properties of the list of variables [xs] by an
+    executable version of this predicate, with a result in [bool]. This way,
+    the tactic [reflexivity] can prove all the desired facts, when the lemma
+    in invoked on a concrete function. We omit the details, and simply
+    state the type of the boolean function [var_fixs_exec]. *)
+
+Parameter var_fixs_exec : var -> vars -> nat -> bool.
+
+(** The second change is to introduce the [wpgen] function in place of
+    the triple for the evaluation of the body of the function. The
+    substitution [substn (f::xs) (v0::vs)] then gets described by the
+    substitution context [List.combine (f::xs) (v0::vs)], which describes
+    a list of pairs of type [list (var * val)].
+
+    The statement of the lemma for [xwp] is as follows. We omit the proof
+    details---they may be found in the implementation of the CFML tool. *)
+
+Parameter xwp_lemma_fixs : forall v0 ts vs f xs t1 H Q,
+  v0 = val_fixs f xs t1 ->
+  trms_to_vals ts = Some vs ->
+  var_fixs_exec f xs (LibList.length vs) ->
+  H ==> (wpgen (combine (f::xs) (v0::vs)) t1) Q ->
+  triple (trm_apps v0 ts) H Q.
+
+(** One last practical details is the set up of the coercion for writing
+    function applications in a concise way. With n-ary functions, the
+    application of a function [f] to two arguments [x] and [y] takes the
+    form [trm_apps f (x::y::nil)]. This syntax is fairly verbose in
+    comparison with the syntax [f x y], which we were able to set up by
+    declaring [trm_app] as a [Funclass] coercion (recall chapter [SLFRules]).
+
+    If we simply declare [trm_apps] as a [Funclass] coercion, we can write
+    [f (x::y::nil)] to denote the application, but we still have to write
+    the list constructors explicitly.
+
+    Fortunately, there is a trick to get the expression [f x y] to be
+    interpreted by Coq as [trm_apps f (x::y::nil)], a trick that works
+    for any number of arguments. The trick is described next. *)
+
+Module NarySyntax.
+
+(** To illustrate the construction, let us consider a simplified grammar
+    of terms that includes the constructor [trm_apps] for n-ary applications. *)
+
+Inductive trm : Type :=
+  | trm_val : val -> trm
+  | trm_apps : trm -> list trm -> trm.
+
+(** We introduce the data type [apps] to represent the syntax tree
+    associated with iterated applications of terms to terms.
+
+    - The application of a term to a term, that is, [t1 t2], gets interpreted
+      via a [Funclass] coercion as [apps_init t1 t2], which is an expression
+      of type [apps].
+    - The application of an object of type [apps] to a term, that is [a1 t2],
+      gets interpreted via another [Funclass] coercion as [apps_next a1 t2].
+
+*)
+
+Inductive apps : Type :=
+  | apps_init : trm -> trm -> apps
+  | apps_next : apps -> trm -> apps.
+
+Coercion apps_init : trm >-> Funclass.
+Coercion apps_next : apps >-> Funclass.
+
+(** For example, the expression [f x y z] gets parsed by Coq as
+    [apps_next (apps_next (apps_init f x) y) z]. From there, the
+    desired term [trm_apps f (x::y::z::nil)] can be computed by a
+    Coq function, called [apps_to_trm], that process the syntax tree
+    of the [apps] expression.
+
+    - In the base case, [apps_init t1 t2] describes the application
+      of a function to one argument: [trm_apps t1 (t2::nil)].
+    - Next, if an apps structure [a1] describes a term [trm_apps t0 ts],
+      then [apps_next a1 t2] describes the term [trm_apps t0 (ts++t2::nil)],
+      that is, an application to one more argument. *)
+
+Fixpoint apps_to_trm (a:apps) : trm :=
+  match a with
+  | apps_init t1 t2 => trm_apps t1 (t2::nil)
+  | apps_next a1 t2 =>
+      match apps_to_trm a1 with
+      | trm_apps t0 ts => trm_apps t0 (List.app ts (t2::nil))
+      | t0 => trm_apps t0 (t2::nil)
+      end
+  end.
+
+(** The function [apps_to_trm] is declared as a coercion from [apps]
+    to [trm], so that any iterated application can be interpreted as
+    the corresponding [trm_apps] term. (Coq raises an "ambiguous coercion
+    path" warning, but this warning may be safely ignored here.) *)
+
+Coercion apps_to_trm : apps >-> trm.
+
+(** The following demo shows how the term [f x y z] is parsed as
+    [apps_to_trm (apps_next (apps_next (apps_init f x) y) z)], which
+    then simplifies by [simpl] to [trm_apps f (x::y::z::nil)]. *)
+
+Lemma apps_demo : forall (f x y z:trm),
+  (f x y z : trm) = trm_apps f (x::y::z::nil).
+Proof using. intros. (* activate display of coercions *) simpl. Abort.
+
+End NarySyntax.
+
+End PrimitiveNaryFun.
 
 
