theories/SLFPreface.v
@@ -156,8 +156,10 @@
     - [SLFWand]:   introduction of the magic wand, of the ramified frame rule,
                    and recursive computation of weakest precondition inside functions.
 
-    - [SLFStruct]: representation predicate for records and arrays, and support
-                   for n-ary functions.
+    - [SLFStruct]: representation predicate for records and arrays.
+
+    - [SLFRich]:   treatment of additional language constructs, including loops,
+                   assertions, and n-ary functions.
 
     - [SLFAffine]: description of a generalized Separation Logic that supports the
                    ability to freely discard certain types of heap predicates.
